lint list progress

Computability/Constructions/List.lean
@@ -87,7 +87,8 @@ def c_list_headI := c_ifz.comp₃ c_id zero (left.comp c_pred)
   by_cases hl : lN=0
   · simp [hl]
   · rw [←(exists_add_one_eq.mpr (one_le_iff_ne_zero.mpr hl)).choose_spec]; simp
-@[simp, ev_simps] theorem c_list_headI_ev {O : ℕ → ℕ} {lN : ℕ} : eval O c_list_headI lN = headI (n2l lN) := by
+@[simp, ev_simps] theorem c_list_headI_ev {O : ℕ → ℕ} {lN : ℕ} :
+    eval O c_list_headI lN = headI (n2l lN) := by
   simp [← evalp_eq_eval c_list_headI_prim]
 end Oracle.Single.Code
 end list_headI
@@ -149,12 +150,12 @@ def c_list_drop :=
     evalp O c_list_drop (Nat.pair i lN) = l2n (drop i (n2l lN)) := by
   simp only [c_list_drop, evp_simps]
   by_cases hl : lN=0
-  · simp only [unpaired, hl, unpair_pair, pair_r, list_ofNat_zero, drop_nil, encode_list_nil]
+  · simp only [unpaired, hl, unpair_pair, list_ofNat_zero, drop_nil, encode_list_nil]
     induction i with
     | zero => simp
     | succ n ih => simp [ih]
   · rw [←(exists_add_one_eq.mpr (one_le_iff_ne_zero.mpr hl)).choose_spec];
-    simp only [unpaired, unpair_pair, pair_r, list_ofNat_succ, unpair1_to_l, ofNat_nat,
+    simp only [unpaired, unpair_pair, list_ofNat_succ, unpair1_to_l, ofNat_nat,
       unpair2_to_r]
     induction i with
     | zero => simp
@@ -194,10 +195,12 @@ section list_getI
 namespace Oracle.Single.Code
 def c_list_getI := c_pred.comp c_list_getElem?
 @[cp] theorem c_list_getI_prim : code_prim c_list_getI := by unfold c_list_getI; apply_cp
-@[simp, evp_simps] theorem c_list_getI_evp {O : ℕ → ℕ} {lN i : ℕ} : evalp O c_list_getI ⟪lN, i⟫ = ((n2l lN).getI i) := by
+@[simp, evp_simps] theorem c_list_getI_evp {O : ℕ → ℕ} {lN i : ℕ} :
+    evalp O c_list_getI ⟪lN, i⟫ = ((n2l lN).getI i) := by
   simp [c_list_getI]
   by_cases hl : i < (n2l lN).length <;> simp [hl, getI]
-@[simp, ev_simps] theorem c_list_getI_ev {O : ℕ → ℕ} {lN i : ℕ} : eval O c_list_getI ⟪lN, i⟫ = ((n2l lN).getI i) := by simp [← evalp_eq_eval c_list_getI_prim]
+@[simp, ev_simps] theorem c_list_getI_ev {O : ℕ → ℕ} {lN i : ℕ} :
+  eval O c_list_getI ⟪lN, i⟫ = ((n2l lN).getI i) := by simp [← evalp_eq_eval c_list_getI_prim]
 end Oracle.Single.Code
 end list_getI
 
@@ -232,7 +235,7 @@ def c_list_foldl_aux (c : Code) :=
   c_list_casesOn' right c_id (pair (c.comp₂ left x) (xs))
 def c_list_foldl_aux2 (c : Code) := (c_nat_iterate (c_list_foldl_aux c)).comp₂ c_id right
 def c_list_foldl (c : Code) := left.comp (c_list_foldl_aux2 c)
-@[cp] theorem c_list_foldl_prim  {c : Code} (hc : code_prim c) : code_prim (c_list_foldl c) := by
+@[cp] theorem c_list_foldl_prim {c : Code} (hc : code_prim c) : code_prim (c_list_foldl c) := by
   rewrite [c_list_foldl, c_list_foldl_aux2, c_list_foldl_aux]; apply_cp
 @[simp, evp_simps] theorem c_list_foldl_aux_evp {O : ℕ → ℕ} {c : Code} {init lN : ℕ} :
     evalp O (c_list_foldl_aux c) ⟪init, lN⟫ =
@@ -253,7 +256,7 @@ def c_list_foldl (c : Code) := left.comp (c_list_foldl_aux2 c)
   -- change goal
   suffices ∀ n,
       (evalp O c.c_list_foldl_aux)^[n] ⟪init, lN⟫ =
-      Nat.pair (((n2l lN).take n).foldl (fun a b => evalp O c ⟪a,b⟫) init) (l2n ((n2l lN).drop n)) by
+      ⟪((n2l lN).take n).foldl (fun a b => evalp O c ⟪a,b⟫) init, l2n ((n2l lN).drop n)⟫ by
     rw [this]
     rw (config := {occs := .pos [1]}) [show lN=(l2n (n2l lN)) from by simp]
     rw [take_of_length_le (length_le_encode _)]
@@ -270,13 +273,8 @@ def c_list_foldl (c : Code) := left.comp (c_list_foldl_aux2 c)
       apply Function.iterate_fixed fixedp
     · simp only [Function.iterate_succ']
       by_cases hl2 : (n2l lN).length ≤ n
-      · simp? [ih, hl2] says
-          simp only [Function.comp_apply, ih, c_list_foldl_aux_evp, ofNat_encode, drop_eq_nil_iff,
-            hl2, ↓reduceIte, pair_eq_pair, encode_inj, drop_eq_drop_iff, inf_of_le_right,
-            right_eq_inf]
-        simp only [take_of_length_le hl2]
-        simp only [take_of_length_le (le_add_right_of_le hl2), true_and]
-        exact le_add_right_of_le hl2
+      · simpa [ih, hl2, take_of_length_le hl2, take_of_length_le (le_add_right_of_le hl2)]
+        using le_add_right_of_le hl2
       · simp? [ih, hl2] says
           simp only [Function.comp_apply, ih, c_list_foldl_aux_evp, ofNat_encode, drop_eq_nil_iff,
           hl2, ↓reduceIte, tail_drop, pair_eq_pair, and_true]
@@ -307,16 +305,18 @@ namespace Oracle.Single.Code
 -- Note that reverse = foldl (flip ( : )) [].
 def c_list_reverse := (c_list_foldl (c_list_cons.comp c_flip)).comp₂ c_list_nil c_id
 @[cp] theorem c_list_reverse_prim : code_prim c_list_reverse := by unfold c_list_reverse; apply_cp
-@[simp, evp_simps] theorem c_list_reverse_evp {O : ℕ → ℕ} {lN} : evalp O c_list_reverse lN =  l2n (reverse (n2l lN)) := by
-  simp only [c_list_reverse]
-  simp [-encode_list_cons, -encode_list_nil]
-  have aux : ∀ l r, foldl (fun (s : ℕ) (b : ℕ) => l2n (b :: (n2l s))) r l = l2n (reverseAux l (n2l r)) := fun l => by
-    induction l with
+@[simp, evp_simps] theorem c_list_reverse_evp {O : ℕ → ℕ} {lN} :
+    evalp O c_list_reverse lN =  l2n (reverse (n2l lN)) := by
+  simp only [c_list_reverse, evp_simps]
+  have aux : ∀ l r,
+      foldl (fun (s : ℕ) (b : ℕ) => l2n (b :: (n2l s))) r l = l2n (reverseAux l (n2l r)) :=
+    fun l => by induction l with
     | nil => simp [*, reverseAux]
     | cons head tail ih => simp [*, reverseAux, -encode_list_cons]
   rw [aux (n2l lN) (l2n [])]
   simp
-@[simp, ev_simps] theorem c_list_reverse_ev {O : ℕ → ℕ} {lN} : eval O c_list_reverse lN =  l2n (reverse (n2l lN)) := by simp [← evalp_eq_eval c_list_reverse_prim]
+@[simp, ev_simps] theorem c_list_reverse_ev {O : ℕ → ℕ} {lN} :
+  eval O c_list_reverse lN =  l2n (reverse (n2l lN)) := by simp [← evalp_eq_eval c_list_reverse_prim]
 end Oracle.Single.Code
 end list_reverse
 
@@ -328,7 +328,8 @@ end list_reverse
 section list_foldr
 namespace Oracle.Single.Code
 def c_list_foldr (c : Code) := (c_list_foldl (c.comp c_flip)).comp₂ left (c_list_reverse.comp right)
-@[cp] theorem c_list_foldr_prim {c : Code} (hc : code_prim c) : code_prim (c_list_foldr c) := by unfold c_list_foldr; apply_cp
+@[cp] theorem c_list_foldr_prim {c : Code} (hc : code_prim c) : code_prim (c_list_foldr c) := by
+  unfold c_list_foldr; apply_cp
 @[simp, evp_simps] theorem c_list_foldr_evp {O : ℕ → ℕ} {c : Code} {init lN : ℕ} :
   evalp O (c_list_foldr c) ⟪init, lN⟫ = foldr
     (fun a b => evalp O c ⟪a,b⟫)
@@ -343,29 +344,37 @@ section list_length
 namespace Oracle.Single.Code
 def c_list_length := (c_list_foldl (succ.comp left)).comp₂ zero c_id
 @[cp] theorem c_list_length_prim : code_prim c_list_length := by unfold c_list_length; apply_cp
-@[simp, evp_simps] theorem c_list_length_evp {O : ℕ → ℕ} {lN : ℕ} : evalp O c_list_length lN = length (n2l lN) := by simp [c_list_length]
-@[simp, ev_simps] theorem c_list_length_ev {O : ℕ → ℕ} {lN : ℕ} : eval O c_list_length lN = length (n2l lN) := by simp [← evalp_eq_eval c_list_length_prim]
+@[simp, evp_simps] theorem c_list_length_evp {O : ℕ → ℕ} {lN : ℕ} :
+  evalp O c_list_length lN = length (n2l lN) := by simp [c_list_length]
+@[simp, ev_simps] theorem c_list_length_ev {O : ℕ → ℕ} {lN : ℕ} :
+  eval O c_list_length lN = length (n2l lN) := by simp [← evalp_eq_eval c_list_length_prim]
 end Oracle.Single.Code
 end list_length
 
 section list_getLast?
 namespace Oracle.Single.Code
 def c_list_getLast? := c_list_getElem?.comp₂ c_id (c_pred.comp <| c_list_length.comp c_id)
-@[cp] theorem c_list_getLast?_prim : code_prim c_list_getLast? := by unfold c_list_getLast?; apply_cp
-@[simp, evp_simps] theorem c_list_getLast?_evp {O : ℕ → ℕ} {lN : ℕ} : evalp O c_list_getLast? lN = o2n (getLast? (n2l lN)) := by
-  simp [c_list_getLast?]
-  exact Eq.symm getLast?_eq_getElem?
-@[simp, ev_simps] theorem c_list_getLast?_ev {O : ℕ → ℕ} {lN : ℕ} : eval O c_list_getLast? lN = o2n (getLast? (n2l lN)) := by simp [← evalp_eq_eval c_list_getLast?_prim]
+@[cp] theorem c_list_getLast?_prim : code_prim c_list_getLast? := by
+  unfold c_list_getLast?; apply_cp
+@[simp, evp_simps] theorem c_list_getLast?_evp {O : ℕ → ℕ} {lN : ℕ} :
+    evalp O c_list_getLast? lN = o2n (getLast? (n2l lN)) := by
+  simpa [c_list_getLast?] using Eq.symm getLast?_eq_getElem?
+@[simp, ev_simps] theorem c_list_getLast?_ev {O : ℕ → ℕ} {lN : ℕ} :
+    eval O c_list_getLast? lN = o2n (getLast? (n2l lN)) := by
+  simp [← evalp_eq_eval c_list_getLast?_prim]
 end Oracle.Single.Code
 end list_getLast?
 
 section list_getLastI
 namespace Oracle.Single.Code
 def c_list_getLastI := c_opt_iget.comp c_list_getLast?
-@[cp] theorem c_list_getLastI_prim : code_prim c_list_getLastI := by unfold c_list_getLastI; apply_cp
-@[simp, evp_simps] theorem c_list_getLastI_evp {O : ℕ → ℕ} {lN : ℕ} : evalp O c_list_getLastI lN = getLastI (n2l lN) := by
+@[cp] theorem c_list_getLastI_prim : code_prim c_list_getLastI := by
+  unfold c_list_getLastI; apply_cp
+@[simp, evp_simps] theorem c_list_getLastI_evp {O : ℕ → ℕ} {lN : ℕ} :
+    evalp O c_list_getLastI lN = getLastI (n2l lN) := by
   simp [c_list_getLastI, getLastI_eq_getLast?_getD]
-@[simp, ev_simps] theorem c_list_getLastI_ev {O : ℕ → ℕ} {lN : ℕ} : eval O c_list_getLastI lN = getLastI (n2l lN) := by simp [← evalp_eq_eval c_list_getLastI_prim]
+@[simp, ev_simps] theorem c_list_getLastI_ev {O : ℕ → ℕ} {lN : ℕ} :
+  eval O c_list_getLastI lN = getLastI (n2l lN) := by simp [← evalp_eq_eval c_list_getLastI_prim]
 end Oracle.Single.Code
 end list_getLastI
 
@@ -377,20 +386,25 @@ section list_append
 namespace Oracle.Single.Code
 def c_list_append := (c_list_foldr (c_list_cons)).comp c_flip
 @[cp] theorem c_list_append_prim : code_prim c_list_append := by unfold c_list_append; apply_cp
-@[simp, evp_simps] theorem c_list_append_evp {O : ℕ → ℕ} {l1N l2N} : evalp O c_list_append ⟪l1N, l2N⟫ = l2n ((n2l l1N) ++ (n2l l2N)) := by
-  simp [c_list_append, -encode_list_cons, -encode_list_nil]
+@[simp, evp_simps] theorem c_list_append_evp {O : ℕ → ℕ} {l1N l2N} :
+    evalp O c_list_append ⟪l1N, l2N⟫ = l2n ((n2l l1N) ++ (n2l l2N)) := by
+  simp only [c_list_append, evp_simps]
   induction (n2l l1N) with
   | nil => simp
   | cons head tail ih => simp [ih, -encode_list_cons, -encode_list_nil]
-@[simp, ev_simps] theorem c_list_append_ev {O : ℕ → ℕ} {l1N l2N} : eval O c_list_append ⟪l1N, l2N⟫ = l2n ((n2l l1N) ++ (n2l l2N)) := by simp [← evalp_eq_eval c_list_append_prim]
+@[simp, ev_simps] theorem c_list_append_ev {O : ℕ → ℕ} {l1N l2N} :
+    eval O c_list_append ⟪l1N, l2N⟫ = l2n ((n2l l1N) ++ (n2l l2N)) := by
+  simp [← evalp_eq_eval c_list_append_prim]
 end Oracle.Single.Code
 end list_append
 
 section list_singleton
 namespace Oracle.Single.Code
 def c_list_singleton (c : Code) := c_list_cons.comp₂ c c_list_nil
-@[cp] theorem c_list_singleton_prim  {c : Code} (hc : code_prim c) : code_prim (c_list_singleton c) := by unfold c_list_singleton; apply_cp
-@[simp, evp_simps] theorem c_list_singleton_evp {O : ℕ → ℕ} {c x} : evalp O (c_list_singleton c) x = l2n ([evalp O c x]) := by
+@[cp] theorem c_list_singleton_prim {c : Code} (hc : code_prim c) :
+  code_prim (c_list_singleton c) := by unfold c_list_singleton; apply_cp
+@[simp, evp_simps] theorem c_list_singleton_evp {O : ℕ → ℕ} {c x} :
+    evalp O (c_list_singleton c) x = l2n ([evalp O c x]) := by
   simp [c_list_singleton]
 end Oracle.Single.Code
 end list_singleton
@@ -399,19 +413,24 @@ section list_concat
 namespace Oracle.Single.Code
 def c_list_concat := c_list_append.comp₂ left (c_list_singleton right)
 @[cp] theorem c_list_concat_prim : code_prim c_list_concat := by unfold c_list_concat; apply_cp
-@[simp, evp_simps] theorem c_list_concat_evp {O : ℕ → ℕ} {lN i : ℕ} : evalp O c_list_concat ⟪lN, i⟫ = l2n ((n2l lN)++[i]) := by
+@[simp, evp_simps] theorem c_list_concat_evp {O : ℕ → ℕ} {lN i : ℕ} :
+    evalp O c_list_concat ⟪lN, i⟫ = l2n ((n2l lN)++[i]) := by
   simp [c_list_concat, -encode_list_cons, -encode_list_nil]
-@[simp, ev_simps] theorem c_list_concat_ev {O : ℕ → ℕ} {lN i : ℕ} : eval O c_list_concat ⟪lN, i⟫ = l2n ((n2l lN)++[i]) := by simp [← evalp_eq_eval c_list_concat_prim]
+@[simp, ev_simps] theorem c_list_concat_ev {O : ℕ → ℕ} {lN i : ℕ} :
+  eval O c_list_concat ⟪lN, i⟫ = l2n ((n2l lN)++[i]) := by simp [← evalp_eq_eval c_list_concat_prim]
 end Oracle.Single.Code
 end list_concat
 
 -- https : //hackage.haskell.org/package/ghc-internal-9.1201.0/docs/src/GHC.Internal.Base.html#map
 section list_map
 namespace Oracle.Single.Code
-def c_list_map (c : Code) := (c_list_foldr (c_list_cons.comp₂ (c.comp left) right)).comp₂ (c_list_nil) (c_id)
-@[cp] theorem c_list_map_prim  {c : Code} (hc : code_prim c) : code_prim (c_list_map c) := by unfold c_list_map; apply_cp
-@[simp, evp_simps] theorem c_list_map_evp {O : ℕ → ℕ} {c : Code} {lN : ℕ} : evalp O (c_list_map c) lN = l2n ((n2l lN).map (evalp O c)) := by
-  simp [c_list_map, -encode_list_cons, -encode_list_nil]
+def c_list_map (c : Code) :=
+  (c_list_foldr (c_list_cons.comp₂ (c.comp left) right)).comp₂ (c_list_nil) (c_id)
+@[cp] theorem c_list_map_prim {c : Code} (hc : code_prim c) : code_prim (c_list_map c) := by
+  unfold c_list_map; apply_cp
+@[simp, evp_simps] theorem c_list_map_evp {O : ℕ → ℕ} {c : Code} {lN : ℕ} :
+    evalp O (c_list_map c) lN = l2n ((n2l lN).map (evalp O c)) := by
+  simp only [c_list_map, evp_simps]
   induction (n2l lN) with
   | nil => simp
   | cons head tail ih => simp [ih, -encode_list_cons, -encode_list_nil]
@@ -433,19 +452,20 @@ def c_list_zipWith_aux (c : Code) :=
   let y   := c_list_headI.comp yys'
   let x   := right
   let acc := left.comp left
-
   let step :=
     c_list_casesOn'
     yys'
     left
     (pair (c_list_cons.comp₂ (c.comp₂ x y) acc) ys')
-
   (c_list_foldl step).comp₂ (pair c_list_nil right) left
 def c_list_zipWith (c : Code) := c_list_reverse.comp <| left.comp (c_list_zipWith_aux c)
 
-@[cp] theorem c_list_zipWith_aux_prim  {c : Code} (hc : code_prim c) : code_prim (c_list_zipWith_aux c) := by unfold c_list_zipWith_aux; apply_cp
-@[cp] theorem c_list_zipWith_prim  {c : Code} (hc : code_prim c) : code_prim (c_list_zipWith c) := by unfold c_list_zipWith; apply_cp
-theorem c_list_zipWith_evp_aux_2 {a b c : List ℕ} {f : ℕ → ℕ → ℕ} (h : a.length ≤ b.length) : zipWith f (b++c) a = zipWith f b a := by
+@[cp] theorem c_list_zipWith_aux_prim {c : Code} (hc : code_prim c) :
+  code_prim (c_list_zipWith_aux c) := by unfold c_list_zipWith_aux; apply_cp
+@[cp] theorem c_list_zipWith_prim {c : Code} (hc : code_prim c) : code_prim (c_list_zipWith c) := by
+  unfold c_list_zipWith; apply_cp
+theorem c_list_zipWith_evp_aux_2 {a b c : List ℕ} {f : ℕ → ℕ → ℕ} (h : a.length ≤ b.length) :
+    zipWith f (b++c) a = zipWith f b a := by
   -- rw `b` => `take a.length b ++ drop a.length b`
   rewrite [(take_append_drop a.length b).symm]
   -- rw `take a.length b ++ drop a.length b ++ c` => `take a.length b ++ (drop a.length b ++ c)`
@@ -455,7 +475,8 @@ theorem c_list_zipWith_evp_aux_2 {a b c : List ℕ} {f : ℕ → ℕ → ℕ} (h
   have aux8 := @zipWith_append ℕ ℕ ℕ f (take a.length b) (drop a.length b) a [] aux7
   simp at aux6 aux8
   simp [aux6, aux8]
-theorem zipWith_flip {α β γ : Type} {f : α → β → γ} {a : List α} {b : List β} : zipWith f a b = zipWith (flip f) b a := by
+theorem zipWith_flip {α β γ : Type} {f : α → β → γ} {a : List α} {b : List β} :
+    zipWith f a b = zipWith (flip f) b a := by
   induction a generalizing b with
   | nil => simp
   | cons _ _ xih =>
@@ -463,33 +484,36 @@ theorem zipWith_flip {α β γ : Type} {f : α → β → γ} {a : List α} {b :
     | nil => simp
     | cons _ _ yih => simp [xih, flip]
 
-theorem c_list_zipWith_evp_aux_1 {a b c : List ℕ} {f : ℕ → ℕ → ℕ} (h : a.length ≤ b.length) : zipWith f a (b++c) = zipWith f a b := by
+theorem c_list_zipWith_evp_aux_1 {a b c : List ℕ} {f : ℕ → ℕ → ℕ} (h : a.length ≤ b.length) :
+    zipWith f a (b++c) = zipWith f a b := by
   rw [zipWith_flip]
   rw (config := {occs := .pos [2]}) [zipWith_flip]
   exact c_list_zipWith_evp_aux_2 h
 
-theorem c_list_zipWith_evp_aux_3 {f : ℕ → ℕ → ℕ} {head} {tail : List ℕ} {l2N head2 list2} (hh : tail.length < (n2l l2N).length) (hl2 : drop tail.length (n2l l2N) = head2 :: list2) : (f head (head2 :: list2).headI :: (zipWith f tail.reverse (n2l l2N)).reverse) = (zipWith f (tail.reverse ++ [head]) (n2l l2N)).reverse := by
-  simp
+theorem c_list_zipWith_evp_aux_3 {f : ℕ → ℕ → ℕ} {head} {tail : List ℕ} {l2N head2 list2}
+    (hh : tail.length < (n2l l2N).length) (hl2 : drop tail.length (n2l l2N) = head2 :: list2) :
+    (f head (head2 :: list2).headI :: (zipWith f tail.reverse (n2l l2N)).reverse) =
+    (zipWith f (tail.reverse ++ [head]) (n2l l2N)).reverse := by
+  simp only [headI_cons]
   have aux5 : (n2l l2N) = (take tail.length (n2l l2N)) ++ [head2] ++ list2 := by
-    -- rw `(n2l l2N)` => `(take tail.length (n2l l2N)) ++ drop tail.length (n2l l2N)`
     rw (config := {occs := .pos [1]}) [Eq.symm (take_append_drop tail.length (n2l l2N))]
     rw [append_assoc, hl2]
     simp
   have aux7 :
-    let l₁ := tail.reverse ++ [head]
-    let l₂ := take tail.length (n2l l2N) ++ [head2] ++ list2
-    let l₁' := zipWith f (tail.reverse) (take tail.length (n2l l2N))
-    let l₂' : List ℕ := [f head head2]
-    ∃ ws xs ys zs, ws.length = ys.length ∧ l₁ = ws ++ xs ∧ l₂ = ys ++ zs ∧ l₁' = zipWith f ws ys ∧ l₂' = zipWith f xs zs := by
-      let ws := tail.reverse
-      let ys := take tail.length (n2l l2N)
-      let xs := [head]
-      let zs := [head2] ++ list2
-      use ws,xs,ys,zs
-      constructor
-      · simp [ws,ys]
-        exact le_of_succ_le hh
-      · exact ⟨rfl, append_assoc (take tail.length (n2l l2N)) [head2] list2, rfl, rfl⟩
+      let l₁ := tail.reverse ++ [head]
+      let l₂ := take tail.length (n2l l2N) ++ [head2] ++ list2
+      let l₁' := zipWith f (tail.reverse) (take tail.length (n2l l2N))
+      let l₂' : List ℕ := [f head head2]
+      ∃ ws xs ys zs, ws.length = ys.length ∧ l₁ = ws ++ xs ∧ l₂ = ys ++ zs ∧ l₁' =
+      zipWith f ws ys ∧ l₂' = zipWith f xs zs := by
+    let ws := tail.reverse
+    let ys := take tail.length (n2l l2N)
+    let xs := [head]
+    let zs := [head2] ++ list2
+    use ws,xs,ys,zs
+    constructor
+    · simpa [ws,ys] using le_of_succ_le hh
+    · exact ⟨rfl, append_assoc (take tail.length (n2l l2N)) [head2] list2, rfl, rfl⟩
   have aux9 : tail.reverse.length ≤ (take tail.length (n2l l2N)).length := by
     simp only [length_reverse, length_take, le_inf_iff, le_refl, true_and]
     exact le_of_succ_le hh
@@ -497,16 +521,14 @@ theorem c_list_zipWith_evp_aux_3 {f : ℕ → ℕ → ℕ} {head} {tail : List �
   rw [zipWith_eq_append_iff.mpr aux7]
   rw (config := {occs := .pos [1]}) [aux5]
   rw [append_assoc (take tail.length (n2l l2N)) [head2] list2]
-  simp
-  exact c_list_zipWith_evp_aux_1 aux9
+  simpa using c_list_zipWith_evp_aux_1 aux9
 theorem c_list_zipWith_aux_evp {O c l1N l2N} :
-  evalp O (c_list_zipWith_aux c) ⟪l1N, l2N⟫
-    =
-  Nat.pair ((zipWith (fun x y => evalp O c ⟪x,y⟫) l1N l2N).reverse) (drop (n2l l1N).length (n2l l2N)) := by
-
+    evalp O (c_list_zipWith_aux c) ⟪l1N, l2N⟫ =
+    Nat.pair
+      ((zipWith (fun x y => evalp O c ⟪x,y⟫) l1N l2N).reverse)
+      (drop (n2l l1N).length (n2l l2N)) := by
   let f := fun x y => evalp O c ⟪x,y⟫
-
-  simp [c_list_zipWith_aux, -encode_list_cons, -encode_list_nil]
+  simp only [c_list_zipWith_aux, evp_simps]
   induction h : (n2l l1N).reverse generalizing l1N with
   | nil => simp_all
   | cons head tail ih =>
@@ -516,11 +538,10 @@ theorem c_list_zipWith_aux_evp {O c l1N l2N} :
       rw [h]
       exact reverse_cons
     rw [asd2]
-
-    simp [-encode_list_cons, -encode_list_nil] at ih
-    simp [-encode_list_cons, -encode_list_nil, -foldl_reverse]
+    simp only [Pi.natCast_apply, cast_id] at ih
     have asdd : (n2l (l2n tail.reverse)).reverse = tail := by simp
     have lolz := ih asdd
+    simp [-encode_list_cons, -encode_list_nil, -foldl_reverse]
     simp [-encode_list_cons, -encode_list_nil, -foldl_reverse] at lolz
     rw [lolz]
     simp [-encode_list_cons, -encode_list_nil, -foldl_reverse]
@@ -537,14 +558,16 @@ theorem c_list_zipWith_aux_evp {O c l1N l2N} :
       -- now we have `drop tail.length (n2l l2N) = head2 :: list2`
       simp only [hl2]
       simp only [drop_eq_nil_iff, not_le] at hh
-      have main : (f head (head2 :: list2).headI :: (zipWith f tail.reverse (n2l l2N)).reverse) = (zipWith f (tail.reverse ++ [head]) (n2l l2N)).reverse := c_list_zipWith_evp_aux_3 hh hl2
+      have main :
+          (f head (head2 :: list2).headI :: (zipWith f tail.reverse (n2l l2N)).reverse) =
+          (zipWith f (tail.reverse ++ [head]) (n2l l2N)).reverse :=
+        c_list_zipWith_evp_aux_3 hh hl2
       rw [main]
 
 @[simp, evp_simps] theorem c_list_zipWith_evp {O : ℕ → ℕ} {c l1N l2N} :
-  evalp O (c_list_zipWith c) ⟪l1N, l2N⟫
-    =
-  zipWith (fun x y => evalp O c ⟪x,y⟫) l1N l2N := by
-    simp [c_list_zipWith, c_list_zipWith_aux_evp]
+    evalp O (c_list_zipWith c) ⟪l1N, l2N⟫ =
+    zipWith (fun x y => evalp O c ⟪x,y⟫) l1N l2N := by
+  simp [c_list_zipWith, c_list_zipWith_aux_evp]
 end Oracle.Single.Code
 end list_zipWith
 
@@ -557,14 +580,16 @@ def c_list_range :=
   (c_list_nil)
   (c_list_concat.comp₂ prev_list i)).comp₂ zero c_id
 @[cp] theorem c_list_range_prim : code_prim c_list_range := by unfold c_list_range; apply_cp
-@[simp, evp_simps] theorem c_list_range_evp {O : ℕ → ℕ} {n} : evalp O c_list_range n = l2n (range n) := by
-  simp [c_list_range, -encode_list_cons, -encode_list_nil]
+@[simp, evp_simps] theorem c_list_range_evp {O : ℕ → ℕ} {n} :
+    evalp O c_list_range n = l2n (range n) := by
+  simp only [c_list_range, evp_simps]
+  simp only [unpaired, encode_list_nil, unpair_pair]
   induction n with
   | zero => simp
   | succ n ih =>
-    simp [-encode_list_cons, -encode_list_nil, ih]
-    exact Eq.symm range_succ
-@[simp, ev_simps] theorem c_list_range_ev {O : ℕ → ℕ} {n} : eval O c_list_range n = l2n (range n) := by simp [← evalp_eq_eval c_list_range_prim]
+    simpa [-encode_list_cons, -encode_list_nil, ih] using Eq.symm range_succ
+@[simp, ev_simps] theorem c_list_range_ev {O : ℕ → ℕ} {n} :
+  eval O c_list_range n = l2n (range n) := by simp [← evalp_eq_eval c_list_range_prim]
 end Oracle.Single.Code
 end list_range
 
@@ -576,15 +601,19 @@ def c_list_replicate :=
   (prec
   (c_list_nil)
   (c_list_concat.comp₂ prev_list x)).comp c_flip
-@[cp] theorem c_list_replicate_prim : code_prim c_list_replicate := by unfold c_list_replicate; apply_cp
-@[simp, evp_simps] theorem c_list_replicate_evp {O : ℕ → ℕ} {n x} : evalp O c_list_replicate ⟪n,x⟫ = l2n (replicate n x) := by
-  simp [c_list_replicate, -encode_list_cons, -encode_list_nil]
+@[cp] theorem c_list_replicate_prim : code_prim c_list_replicate := by
+  unfold c_list_replicate; apply_cp
+@[simp, evp_simps] theorem c_list_replicate_evp {O : ℕ → ℕ} {n x} :
+    evalp O c_list_replicate ⟪n,x⟫ = l2n (replicate n x) := by
+  simp only [c_list_replicate, evp_simps]
+  simp only [unpaired, encode_list_nil, unpair_pair]
   induction n with
   | zero => simp
   | succ n ih =>
-    simp [-encode_list_cons, -encode_list_nil, ih]
-    exact Eq.symm replicate_succ'
-@[simp, ev_simps] theorem c_list_replicate_ev {O : ℕ → ℕ} {n x} : eval O c_list_replicate ⟪n,x⟫ = l2n (replicate n x) := by simp [← evalp_eq_eval c_list_replicate_prim]
+    simpa [-encode_list_cons, -encode_list_nil, ih] using Eq.symm replicate_succ'
+@[simp, ev_simps] theorem c_list_replicate_ev {O : ℕ → ℕ} {n x} :
+    eval O c_list_replicate ⟪n,x⟫ = l2n (replicate n x) := by
+  simp [← evalp_eq_eval c_list_replicate_prim]
 end Oracle.Single.Code
 end list_replicate
 
@@ -596,24 +625,22 @@ namespace Oracle.Single.Code
 def c_list_map' (c : Code) :=
   let lN := left
   let aux := right
-  (c_list_map c).comp ((c_list_zipWith c_id).comp₂ lN (c_list_replicate.comp₂ (c_list_length.comp lN) aux))
+  (c_list_map c).comp
+  ((c_list_zipWith c_id).comp₂ lN (c_list_replicate.comp₂ (c_list_length.comp lN) aux))
 @[cp] theorem c_list_map'_prim {c : Code} (hc : code_prim c) : code_prim (c_list_map' c) := by
   unfold c_list_map'; apply_cp
 @[simp, evp_simps] theorem c_list_map'_evp {O : ℕ → ℕ} {c lN aux} :
-  evalp O (c_list_map' c) ⟪lN, aux⟫
-    =
-  ((n2l lN).map (fun ele => evalp O c (Nat.pair ele aux))) := by
-  simp only [c_list_map', evp_simps, ]
-  simp only [pair_l, pair_r, ofNat_encode, map_zipWith, encode_inj]
+    evalp O (c_list_map' c) ⟪lN, aux⟫ =
+    ((n2l lN).map (fun ele => evalp O c (Nat.pair ele aux))) := by
+  simp only [c_list_map', evp_simps]
+  simp only [ofNat_encode, map_zipWith, encode_inj]
   induction (n2l lN) with
   | nil => simp [Nat.pair]
-  | cons head tail ih =>
-    simp only [length_cons, replicate_succ, zipWith_cons_cons, map_cons, cons.injEq, true_and];
-    exact ih
+  | cons head tail ih => simpa [replicate_succ] using ih
 end Oracle.Single.Code
 end list_map'
 
-@[simp] theorem getLastI_append {x} {y : ℕ}: (x++[y]).getLastI = y := by
+@[simp] theorem getLastI_append {x} {y : ℕ} : (x++[y]).getLastI = y := by
   simp [getLastI_eq_getLast?_getD]
 
 /-
@@ -668,9 +695,7 @@ lemma c_list_foldr_param_aux_2 {f : ℕ → ℕ} {param init lst} :
       init
       lN.n2l
     ) := by
-  simp only [c_list_foldr_param_aux, evp_simps]
-  simp only [pair_l, pair_r, ofNat_encode]
-  exact c_list_foldr_param_aux_2
+  simpa [c_list_foldr_param_aux, evp_simps] using c_list_foldr_param_aux_2
 @[simp, evp_simps] theorem c_list_foldr_param_evp {O : ℕ → ℕ} {c param init lN} :
   evalp O (c_list_foldr_param c) ⟪param, init, lN⟫ =
   foldr
